\subsection{Tensions in Cosmology}
Define the posterior probability of parameters $\theta$ within model $\mathcal{M}$ given data $d$ as (Bayes' theorem)
\begin{equation}
    \mathcal{P}(\theta) := P(\theta|d,\mathcal{M}) = \frac{P(\theta|\mathcal{M})P(d|\theta,\mathcal{M})}{P(d|\mathcal{M})}
\end{equation}
The following notation will simplify this expression
\begin{equation*}
    \begin{split}
        \Pi(\theta) &= P(\theta|\mathcal{M}) \text{ , Prior probability} \\
        \mathcal{L}(\theta) &= P(d|\theta,\mathcal{M}) \text{ , the likelihood} \\
        \mathcal{E} &= P(d|\mathcal{M}) \text{ , the evidence}
    \end{split}
\end{equation*}
$$     \mathcal{P}(\theta) := P(\theta|d,\mathcal{M}) = \frac{\Pi(\theta)\mathcal{L}}{\mathcal{E}} $$
These are (maybe?) understandable as the prior probability is the parameters given the model, the likelihood as the data given some parameters of the model, and the evidence as the data give a model. From now on, the model $\mathcal{M}$ will be implied.

Consider now two data sets $d_1,d_2$. They have a joint likelihood $$\mathcal{L}(\theta) = P(d_1,d_2|\theta)$$
This \textbf{quantifies the likelihood of $d_1$ and $d_2$ coming from the same set of parameters of a given model.} Denote now $\mathcal{L}_1,\mathcal{P}_1$ as the marginalized likelihood and Posterior over $d_2$. (\textbf{Is there a procedure/algorithm to find the marginalized probability? Seems generally non-trivial}).

Now duplicate the parameter set to $\theta_1,\theta_2$ and perscibe a new joint likelihood $\mathcal{L}(\theta_1,\theta_2) = P(d_1,d_2|\theta_1,\theta_2)$.\textbf{ This is generally a choice, but how can one make a good choice?} The choice however is not unique.

As such, the constraints are imposed:
\begin{enumerate}
    \item $\mathcal{L}(\theta_1=\theta,\theta_2=\theta) = \mathcal{L}(\theta)$, or in plain english, the joint likelihood if $\theta_1=\theta=\theta_2$ needs to coincide with the likelihood of $\theta$
    \item $P(d_1|\theta_1,\theta_2)=P(d_1|\theta_1)$ once marginalized over $d_2$. Marginalizing the likelihood over one of the data sets removes the dependancy on the corresponding parameter sets.
\end{enumerate}
 \textbf{This ensures the datasets are conditionally independent,}
    $$ P(d_1,d_2|\theta) = P(d_1|\theta)P(d_2|\theta)$$
\textbf{Proof?}
Which means we can choose $$\mathcal{L}(\theta_1,\theta_2) = \mathcal{L}_1(\theta_1)\mathcal{L}_2(\theta_2)$$
If we further assume the prior distribution can be factorized, the joint posterior is then
$$ \mathcal{P}(\theta_1,\theta_2) = \mathcal{L}(\theta_1,\theta_2)\Pi(\theta_1)\Pi(\theta_2) $$
Defining $\Delta\theta = \theta_1-\theta_2$, the parameter difference posterior is given by
\[ \mathcal{P}(\Delta\theta) = \int_{V_\Pi} \mathcal{P}(\theta,\theta-\Delta\theta)d\theta\]

\subsection{Quantifying Results}

Given some probability $P$ of a parameter shift, the following formula can give you the number of standard deviations if the probability shift comes from a gaussian distribution
\[ n_\sigma = \sqrt{2} \text{Erf}^{-1}(P) \]
I have a notebook using two unit gaussian priors separated by a distance $a$. This example can be computed analytically.
\begin{equation*}
    \begin{split}
	\mathcal{P}(\Delta \theta) &= \frac{1}{2\pi} \int\limits_{-\infty}^{\infty} e^{-\theta^2/2} e^{-(\theta-\Delta\theta)^2/2}  d\theta \\
				   &= \frac{1}{2\pi} \cdot \sqrt{\pi} e^{-(\Delta\theta)^2/4}\\
				   &= \frac{1}{\sqrt{4\pi}}e^{-(\Delta\theta)^2/4}\\
    \end{split}
\end{equation*}
The parameter difference posterior is a gaussian with standard deviation $\sqrt{2}$. The separation is fixed by $a$, hence the shift is $\mathcal{P}(a)$. Hence the shift probability is
\[ \Delta = \int\limits_{-a}^{a} e^{-(\Delta\theta)^2/4} d\Delta\theta \]
Lets use the example $a=2$. Then $n_\sigma = 2/\sqrt{2} = \sqrt{2}$. Using this we can work backwards to find $\Delta$ from a $z$-table to find $\Delta = 0.9207 - 0.0793 = 0.8414 $. 
